Cm/Pi/Infer2.lean
@@ -1,0 +1,131 @@
+import Cm.Pi.Std.Except
+import Cm.Pi.Eval
+import Cm.Pi.Ast
+
+open Expr
+
+def TData : Expr := .symbol "Data"
+
+def TFail : Expr := .symbol "sorry"
+
+def expected_but_found : Expr :=
+  (λ' 1 (λ' 2 (::
+    (λ' 1 (::
+      (var.store 1)
+      (λ' 1 (:: (:: (var.store 0) <| symbol "expected:") (var.read 0)))))
+        (:: (var.store 0) <| (λ' 1 (:: (:: (var.store 0) <| symbol "but found: ") (var.read 0)))))))
+
+def assert_eq : Expr :=
+  let my_v := var.read 0
+
+  let eq_ok := (λ' 1 (:: (var.store 1) (λ' 1 (:: (:: (var.store 0) Except'.s_ok) my_v))))
+
+  (λ' 1
+    (:: (λ' 1 (:: (:: (var.store 0) eq) (λ' 1 (:: eq_ok
+        (λ' 1 (λ' 2 (:: (:: (var.store 0) (:: (var.store 0) Except'.s_err))
+        (λ' 1 (:: (:: (var.store 0) apply) (λ' 1 (:: (:: (var.store 0) expected_but_found) my_v)))))))))))
+      my_v))
+
+/-
+assert_eq but it returns just the data in the ok case.
+-/
+def assert_eq_unwrap : Expr :=
+  let my_v := var.read 0
+
+  (λ' 1
+    (:: (λ' 1 (:: (:: (var.store 0) eq) (λ' 1 (:: (λ' 1 (:: (var.store 1) my_v))
+      (λ' 1
+        (λ' 2 (::
+          (:: (var.store 0) (:: (var.store 0) Except'.s_err))
+          (λ' 1 (::
+            (:: (var.store 0) apply)
+            (λ' 1 (::
+              (:: (var.store 0) expected_but_found)
+              my_v)))))))))))
+      my_v))
+
+def infer.self : Expr :=
+  :: π (:: id nil)
+
+def infer.x (with_op : Expr := id) : Expr :=
+  :: π (:: nil with_op)
+
+
+def infer_nil : Expr :=
+  (λ' 1 (:: (quote apply)
+    (:: π (::
+    (quote <|
+      :: (:: eq (:: (quote <| (:: apply (:: Except'.ok TData))) (:: apply (:: expected_but_found nil))))
+      .nil)
+    id))))
+
+example : try_step_n' 100 (:: apply (:: infer_nil (:: infer_nil nil))) = (.ok (:: Except'.s_ok TData)) := rfl
+
+/-
+Infer fully applied id.
+Curry this for partial app.
+
+Currying = dependent type.
+
+(:: apply (:: infer (:: infer (:: id x)))) = (:: apply (:: infer (:: infer x)))
+-/
+def infer_id : Expr :=
+  :: both (:: (quote apply)
+    (:: both (::
+      (:: π (:: id nil))
+      (:: π (:: id id)))))
+
+example : try_step_n' 100 (:: apply (:: infer_id (:: infer_nil nil))) = (.ok (:: Except'.s_ok TData)) := rfl
+
+/-
+Also fully applied.
+(:: apply (:: infer (:: infer (:: (:: both (:: f g)) x)))) = (:: apply (:: Except'.bothM (:: (:: apply (:: infer (:: infer (:: f x)))) (:: apply (:: infer (:: infer (:: g x)))))))
+-/
+def infer_both.infer_f : Expr :=
+  :: both (:: (quote apply) (:: both (::
+    infer.self (:: π (:: id (:: π (:: id (:: π (:: nil id)))))))))
+
+def infer_both.infer_g : Expr :=
+  :: both (:: (quote apply) (:: both (::
+    infer.self (:: π (:: id (:: π (:: nil (:: π (:: id id)))))))))
+
+def infer_both : Expr :=
+  (:: both (:: (quote apply) (:: both (::
+    (quote Except'.bothM) (:: both (::
+      infer_both.infer_f
+      infer_both.infer_g))))))
+
+def assert_op (op_getter : Expr) : Expr :=
+  (:: π (:: id (:: π (:: op_getter id))))
+
+def assert_whole (whole : Expr) : Expr :=
+  (:: π (:: id whole))
+
+def match_infer (match_fn then_do : Expr) (or_else : Expr := (quote (:: apply (:: Except'.err TFail)))) : Expr :=
+  (:: both (:: (quote apply)
+    (:: both (::
+      (:: both (:: (:: both (:: (quote eq) (:: both (::
+        (quote then_do)
+        (quote or_else)))))
+        match_fn))
+     id))))
+
+def infer_fn' (fn : Expr) : Expr :=
+  (:: both (:: (quote apply) (:: both (::
+    (:: both (:: (quote apply) (:: both (::
+      fn (:: both (::
+      infer.self
+      (:: π (:: nil (:: π (:: id nil))))))))))
+      (:: π (:: nil (:: π (:: nil id))))))))
+
+def infer : Expr :=
+  match_infer
+    (assert_whole (quote nil))
+    infer_nil
+    (match_infer
+      (assert_whole (quote id))
+      (:: both (:: (quote apply) (:: both (:: (quote (:: apply (:: curry infer_id))) infer.self))))
+      (infer_fn' infer.self))
+
+set_option maxRecDepth 5000
+example : try_step_n' 500 (:: apply (:: infer (:: infer (:: id nil)))) = (.ok (:: Except'.s_ok TData)) := rfl
